implemented `ITree.bind`

LeanBoogie/ITree/ITree.lean
@@ -48,52 +48,58 @@ end Internal
 abbrev Ans : Type := Int
 
 def ITree E A := Internal.ITree Ans E A
+
+namespace ITree
+
 -- QPF gotcha: The parameters to ITree get reordered in the ctors somehow
-def ITree.ret {E A} (r : A) : ITree E A := @Internal.ITree.ret A Ans E r
-def ITree.tau {E A} (t : ITree E A) : ITree E A := @Internal.ITree.tau Ans E A t
-def ITree.vis {E A} (e : E) (k : Ans -> ITree E A) := @Internal.ITree.vis E Ans A e k
+def ret {E A} (r : A) : ITree E A := @Internal.ITree.ret A Ans E r
+def tau {E A} (t : ITree E A) : ITree E A := @Internal.ITree.tau Ans E A t
+def vis {E A} (e : E) (k : Ans -> ITree E A) := @Internal.ITree.vis E Ans A e k
 
-abbrev ITree.Base E A β := Internal.ITree.Base Ans E A β
+abbrev Base E A β := Internal.ITree.Base Ans E A β
 
-def ITree.corec {E A β : Type} (f : β → ITree.Base E A β) (b : β) : ITree E A :=
-  MvQPF.Cofix.corec (n := 2) (F := TypeFun.ofCurried (ITree.Base)) f b
+def corec {E A β : Type} (f : β → ITree.Base E A β) (b : β) : ITree E A
+  := MvQPF.Cofix.corec (n := 2) (α := (Vec.reverse (Vec.nil.append1 A ::: E))) (F := TypeFun.ofCurried (n := 3) (ITree.Base)) f b
 
-/-- Execute a finite amount of steps of a potentially infinite ITree.
+def dest {E A : Type} : ITree E A -> ITree.Base E A (ITree E A)
+  := MvQPF.Cofix.dest
+
+@[cases_eliminator, elab_as_elim]
+def cases {E A : Type} {motive : ITree E A → Sort u}
+    (ret : (r : A) → motive (.ret r))
+    (tau : (x : ITree E A) → motive (.tau x))
+    (vis : (e : E) → (k : Ans → ITree E A) → motive (.vis e k)) :
+    ∀ (x : ITree E A), motive x :=
+  fun x =>
+    match h : MvQPF.Cofix.dest x with
+    | .ret r =>
+      have h : x = .ret r := by
+        apply_fun MvQPF.Cofix.mk at h
+        simpa [MvQPF.Cofix.mk_dest] using h
+      h ▸ ret r
+    | .tau y =>
+      have h : x = .tau y := by
+        apply_fun MvQPF.Cofix.mk at h
+        simpa [MvQPF.Cofix.mk_dest] using h
+      h ▸ tau y
+    | .vis e k =>
+      have h : x = .vis e k := by
+        apply_fun MvQPF.Cofix.mk at h
+        simpa [MvQPF.Cofix.mk_dest] using h
+      h ▸ vis e k
+
+/-- Execute a finite amount of steps of a potentially infinite
   Returns the events encountered along the way (if any), and the final state (if any).
   Uses `f` to determine the answer to events. -/
-def ITree.run (t : ITree E A) (f : E -> Ans) : Nat -> (List E) × Option A
+def run (t : ITree E A) (f : E -> Ans) : Nat -> (List E) × Option A
 | 0 => ([], none)
-| n+1 => match MvQPF.Cofix.dest t with
+| n+1 => match t.dest with
   | .ret a => ([], some a)
   | .tau t => run t f n
   | .vis e k => by
     let t : ITree E A := k (f e)
     let (evs, ret) := run t f n
     exact (e :: evs, ret)
-
-@[cases_eliminator, elab_as_elim]
-def ITree.cases {E A : Type} {motive : ITree E A → Sort u}
-    (ret : (r : A) → motive (.ret r))
-    (tau : (x : ITree E A) → motive (ITree.tau x))
-    (vis : (e : E) → (k : Ans → ITree E A) → motive (.vis e k)) :
-    ∀ (x : ITree E A), motive x :=
-  fun x =>
-    match h : MvQPF.Cofix.dest x with
-    | .ret r =>
-      have h : x = ITree.ret r := by
-        apply_fun MvQPF.Cofix.mk at h
-        simpa [MvQPF.Cofix.mk_dest] using h
-      h ▸ ret r
-    | .tau y =>
-      have h : x = ITree.tau y := by
-        apply_fun MvQPF.Cofix.mk at h
-        simpa [MvQPF.Cofix.mk_dest] using h
-      h ▸ tau y
-    | .vis e k =>
-      have h : x = ITree.vis e k := by
-        apply_fun MvQPF.Cofix.mk at h
-        simpa [MvQPF.Cofix.mk_dest] using h
-      h ▸ vis e k
 
 -- # Experimentation:
 
@@ -103,8 +109,8 @@ namespace WithSigma
   | tau (t : ι) -- ι = ITree ε ρ
   | vis (e : ν) -- ν = Σ α : Type, ε α × α → ITree ε ρ
 
-  -- qpf F ε ρ ι ν    = (Σ α : Type, ε α × α → ι)
-  -- qpf F (α : Type) ε ρ ι ν    = Sigma G
+  -- qpf F ε ρ ι ν    := (Σ α : Type, ε α × α → ι)
+  -- qpf F (α : Type) ε ρ ι ν    := Sigma G
 
   qpf G (α : Type) (ε : Type → Type) ρ ι ν := ε α × (α → ι)
 
