LeanBoogie/ITree/Mem.lean
@@ -22,5 +22,52 @@ abbrev Mem : Type -> Type := ITree MemEv
 def Mem.set (a : String) (b : Int) : Mem Unit := .vis (.write a b) (fun _unit => .ret ())
 def Mem.get (v : String)           : Mem Int  := .vis (.read v) (fun ans => .ret ans)
 
--- TODO: interpreting memory events away into the boogie state monad.
--- def interp (handler : MemEv -> Boog Int) (t : Mem A) : Boog A :=
+abbrev Mem.inc (v : String) : Mem Unit := do
+  let x <- get v
+  set v (x+1)
+
+/-
+  # Interpreting memory
+-/
+
+/-- Transforms memory events into state monad actions. -/
+-- def interp (tm : ITree MemEv A) (s₀ : BoogieState) : ITree Empty (A × BoogieState) :=
+def interp (tm : ITree MemEv A) : StateT BoogieState (ITree Empty) A := fun s₀ =>
+  ITree.corec (fun ⟨tm, s⟩ =>
+    match tm.dest with
+    | .ret a => .ret (a, s)
+    | .tau t => .tau (t, s)
+    | .vis (.read v)      k =>
+      let ⟨val, s'⟩ := Boog.get v s
+      .tau ⟨k val, s'⟩
+    | .vis (.write v val) k =>
+      let ⟨(), s'⟩ := Boog.set v (pure val) s
+      .tau ⟨k (default), s'⟩ -- TODO: Instead of `default : Int`, this should be `() : Unit` once the QPF ITree limitation is gone.
+  ) (tm, s₀)
+
+def writeForever : ITree MemEv Empty
+  := ITree.corec (fun a => .vis (MemEv.write "x" 1) (fun _unit => a) ) 0
+
+-- ? If it terminates, can you extract the state transition function?
+#check fun s₀ => ITree.run (interp (Mem.inc "x") s₀) 0 2 |>.2
+-- #eval ITree.run (interp (Mem.inc "x") {}) 0 2 |>.2
+
+#check interp writeForever
+#check ITree.run (interp writeForever {}) 0 0
+#reduce ITree.run (interp writeForever {}) 0 0
+
+theorem interp_ret : interp (.ret x) s = .ret (x, s) := by
+  rw [interp]
+  sorry
+
+
+section Experiment
+-- ## Crazy idea, what if...
+
+def interp_crazy (t : ITree MemEv A) : ITree Empty (A × (BoogieState -> BoogieState -> Prop)) :=
+  match t.dest with
+  | .ret r => .ret (r, (. = .))
+  | .tau r => sorry
+  | .vis e k => sorry
+
+end Experiment
