LeanBoogie/ITree/Monad.lean
@@ -1,45 +1,68 @@
 import LeanBoogie.ITree.ITree
 import LeanBoogie.ITree.Eutt
 
+namespace ITree
+
 /-
   # `ITree` forms a monad
 -/
 
-def ITree.pure (a : A) : ITree E A := .ret a
+def pure (a : A) : ITree E A := .ret a
 
-def ITree.bind (ta : ITree E A) (tb : A -> ITree E B) : ITree E B :=
-  ITree.corec (fun ta => ta.cases
-    (fun (a : A) =>
-      let tb : ITree E B := tb a
-
-      sorry
-    ) -- :(
-    (fun ta => .tau ta)
-    (fun e k => .vis e (fun x => k x))
-  ) ta
+def bind (ta : ITree E A) (tb : A -> ITree E B) : ITree E B :=
+  ITree.corec (β := Sum (ITree E A) (ITree E B)) (fun x =>
+    match x with
+    | .inl ta =>
+      match ta.dest with
+      | .ret (a : A) =>
+        let tb : ITree E B := tb a
+        let tbdest : ITree.Base E B (ITree E B) := tb.dest
+        have : TypeFun.ofCurried Base ((Vec.reverse (Vec.nil.append1 B ::: E)).append1 (ITree E B)) = Base E B (ITree E B) := rfl
+        let INR : TypeVec.Arrow
+          ((Vec.reverse (Vec.nil.append1 B ::: E)).append1 (ITree E B))
+          ((Vec.reverse (Vec.nil.append1 B ::: E)).append1 (ITree E A ⊕ ITree E B))
+          := TypeVec.appendFun TypeVec.id Sum.inr
+        let ret : ITree.Base E B (ITree E A ⊕ ITree E B) := MvFunctor.map (F := TypeFun.ofCurried (n := 3) ITree.Base) INR (this ▸ tbdest)
+        ret
+      | .tau t => .tau (.inl t)
+      | .vis e k => .vis e (fun x => .inl (k x))
+    | .inr b =>
+      match b.dest with
+      | .ret (b : B) => .ret b
+      | .tau t => .tau (.inr t)
+      | .vis e k => .vis e (fun x => .inr (k x))
+  ) (Sum.inl ta)
 
 instance : Monad (ITree E) where
-  pure := ITree.pure
-  bind := ITree.bind
+  pure := pure
+  bind := bind
 
-#check LawfulMonad
+instance : LawfulFunctor (ITree E) where
+  map_const := sorry
+  id_map := sorry
+  comp_map := sorry
+instance : LawfulMonad (ITree E) where
+  seqLeft_eq := sorry
+  seqRight_eq := sorry
+  pure_seq := sorry
+  bind_pure_comp := sorry
+  bind_map := sorry
+  pure_bind := sorry
+  bind_assoc := sorry
 
 /- ## Helpers for writing imperative programs -/
 
-def ITree.skip : ITree E Unit := .ret ()
-def ITree.spin : ITree E A := ITree.corec (fun n => .tau n) 0
-def ITree.seq (a b : ITree E Unit) : ITree E Unit := bind a (fun () => b)
-def ITree.trigger (e : E) : ITree E Int := .vis e (fun ans => .ret ans)
+def skip : ITree E Unit := .ret ()
+def spin : ITree E A := corec (fun n => .tau n) 0
+def seq (a b : ITree E Unit) : ITree E Unit := bind a (fun () => b)
+def trigger (e : E) : ITree E Int := .vis e (fun ans => .ret ans)
+def ite (c : ITree E Bool) (t e : ITree E Unit) : ITree E Unit := bind c (fun c => if c then t else e)
+abbrev ifthen (c : ITree E Bool) (t : ITree E Unit) : ITree E Unit := ite c t skip
 
-def ITree.ite (c : ITree E Bool) (t e : ITree E Unit) : ITree E Unit
-  := bind c (fun c => if c then t else e)
+def assume (φ : Prop) [Decidable φ] : ITree E Unit := if φ then skip else spin
 
-abbrev ITree.ifthen (c : ITree E Bool) (t : ITree E Unit) : ITree E Unit
-  := ite c t skip
 
-def ITree.assume (φ : Prop) [Decidable φ] : ITree E Unit := if φ then skip else spin
-
-/-
+/- # Iter
   From the ITrees paper, page 12:
   CoFixpoint iter (body : A → itree E (A + B)) : A → itree E B :=
     fun a ⇒ ab <- body a ;;
@@ -57,27 +80,26 @@ def ITree.assume (φ : Prop) [Decidable φ] : ITree E Unit := if φ then skip el
       end) (inr a).
 -/
 
--- -- ! Wait,... we don't have loops. We just have blocks.
--- def loop (step : A -> ITree E (Sum A B)) (a : A) : ITree E B :=
---   sorry
+/-- Repeat a computation until it returns `B`. -/
+def iter (body : A -> ITree E (Sum A B)) (a : A) : ITree E B := sorry
+--   ITree.corec (β := Sum A Unit) (fun x =>
+--     match x with
+--     | .inl a =>
+--       let res := bind (body a) (fun ab =>
+--         match ab with
+--         | .inl a => sorry
+--         | .inr b => sorry
+--       )
+--       match res.dest with
+--       | .ret a => sorry
+--       | .tau a => sorry
+--       | .vis e k => sorry
+--       -- | .vis e k => .vis e (fun x => .inl (k x))
+--     | .inr b =>
+--       match b.dest with
+--       | .ret (b : B) => .ret b
+--       | .tau t => .tau (.inr t)
+--       | .vis e k => .vis e (fun x => .inr (k x))
+--   ) (Sum.inl a)
 
--- /--
---         iter step a  : ITree E B
---   step (iter step a) : ITree E B
--- -/
--- def iter (step : A -> ITree E (Sum A B)) (a : A) : ITree E B :=
---   ITree.corec (fun iter_ =>
---     bind (step iter_) (fun
---       | .inl a => step a
---       | .inr b => .ret (.inr b)
---     )
---   ) a
---   -- ITree.corec (fun
---   --   | .inl a => .tau (step a)
---   --   | .inr b => .ret b
---   -- ) (Sum.inl a)
-
---   -- ITree.bind (step a) (fun
---   --   | .inl a => step a
---   --   | .inr b => sorry
---   -- )
+def loop (body : Sum C A -> ITree E (Sum C B)) (a : A) : ITree E B := sorry
